Customised printing of boxes; more Elm tests

extraction/examples/ElmExtractTests.v
@@ -8,6 +8,7 @@ From ConCert.Extraction Require Import MidlangExtract.
 From ConCert.Extraction Require Import Optimize.
 From ConCert.Extraction Require Import PrettyPrinterMonad.
 From ConCert.Extraction Require Import ResultMonad.
+From ConCert.Extraction Require Import StringExtra.
 From ConCert.Extraction Require Import MidlangExtractTests.
 From Coq Require Import Arith.
 From Coq Require Import String.
@@ -21,14 +22,25 @@ From MetaCoq Require Import utils.
 
 Import MonadNotation.
 
-Definition wrapped (p : program) (pre post : string) : result string string :=
+Instance ElmBoxes : BoxSymbol :=
+  {| term_box_symbol := "()"; (* the inhabitant of the unit type *)
+     type_box_symbol := "()"; (* unit type *)
+     any_type_symbol := "()"(* unit type *) |}.
+
+
+Definition general_wrapped (p : program) (pre post : string)
+  (ignore: list kername) (TT : list (kername * string)) : result string string :=
   entry <- match p.2 with
            | tConst kn _ => ret kn
            | _ => Err "Expected program to be a tConst"
            end;;
-  Σ <- specialize_erase_debox_template_env p.1 [entry] [];;
-  '(_, s) <- finish_print (print_env Σ p.1 (fun _ => None));;
+  Σ <- specialize_erase_debox_template_env p.1 [entry] ignore;;
+  let TT_fun kn := option_map snd (List.find (fun '(kn',v) => eq_kername kn kn') TT) in
+  '(_, s) <- finish_print (print_env Σ p.1 TT_fun);;
   ret (pre ++ nl ++ s ++ nl ++ post).
+
+Definition wrapped (p : program) (pre post : string) : result string string :=
+  general_wrapped p pre post [] [].
 
 Module ElmExamples.
   Definition Preambule mod_name :=
@@ -38,29 +50,74 @@ Module ElmExamples.
                   "import Html";
                   "import Expect exposing (Expectation)"].
 
+  Definition elm_false_rec :=
+    String.concat nl
+                  ["false_rec : () -> a";
+                   "false_rec _ = false_rec ()"].
+
   Definition main_and_test (test : string) :=
     "main = Html.text "++ parens false ("Debug.toString " ++ parens false test) ++ nl ++
     "suite = Test.test (Debug.toString 1)" ++ parens false ("\ _ -> " ++ test).
 
+  MetaCoq Quote Recursively Definition rev_syn := List.rev.
+
+  Redirect "./extraction/examples/elm-extract/Rev.elm" Compute wrapped rev_syn
+          (Preambule "Rev")
+          (main_and_test "Expect.equal (rev (Cons 3 (Cons 2 (Cons 1 (Cons 0 Nil))))) (Cons 0 (Cons 1 (Cons 2 (Cons 3 Nil))))").
+
+
+  MetaCoq Quote Recursively Definition nth_syn := List.nth.
+
+  Definition result_nth :=
+    <$ "type Nat";
+       "  = O";
+       "  | S Nat";
+       "";
+       "type List a";
+       "  = Nil";
+       "  | Cons a (List a)";
+       "";
+       "nth : Nat -> List a -> a -> a";
+       "nth n l default =";
+       "  case n of";
+       "    O ->";
+       "      case l of";
+       "        Nil ->";
+       "          default";
+       "        Cons x l2 ->";
+       "          x";
+       "    S m ->";
+       "      case l of";
+       "        Nil ->";
+       "          default";
+       "        Cons x t ->";
+       "          nth m t default" $>.
+
+  Example ElmExamples_nth :
+    extract nth_syn = Ok result_nth.
+  Proof. reflexivity. Qed.
+
+  Redirect "./extraction/examples/elm-extract/Nth.elm" Compute wrapped nth_syn
+          (Preambule "Nth")
+          (main_and_test "Expect.equal (nth O (Cons 1 (Cons 0 Nil)) 0) 1").
+
   MetaCoq Quote Recursively Definition map_syn := List.map.
   Definition result_map :=
-    String.concat nl
-      ["type List a";
-      "  = Nil";
-      "  | Cons a (List a)";
-        "";
-      "map : (a -> b) -> List a -> List b";
-      "map f =";
-      "  let";
-      "    map2 l =";
-      "      case l of";
-      "        Nil ->";
-      "          Nil";
-      "        Cons a t ->";
-      "          Cons (f a) (map2 t)";
-      "  in";
-      "  map2"].
-
+    <$ "type List a";
+       "  = Nil";
+       "  | Cons a (List a)";
+         "";
+       "map : (a -> b) -> List a -> List b";
+       "map f =";
+       "  let";
+       "    map2 l =";
+       "      case l of";
+       "        Nil ->";
+       "          Nil";
+       "        Cons a t ->";
+       "          Cons (f a) (map2 t)";
+       "  in";
+       "  map2" $>.
 
   Redirect "./extraction/examples/elm-extract/Map.elm" Compute wrapped map_syn
           (Preambule "Map")
@@ -72,8 +129,7 @@ Module ElmExamples.
 
   MetaCoq Quote Recursively Definition foldl_syn := List.fold_left.
   Definition result_foldl :=
-    String.concat nl
-      ["type List a";
+  <$ "type List a";
       "  = Nil";
       "  | Cons a (List a)";
         "";
@@ -87,7 +143,7 @@ Module ElmExamples.
       "        Cons b t ->";
       "          fold_left2 t (f a0 b)";
       "  in";
-      "  fold_left2"].
+      "  fold_left2" $>.
 
   Redirect "./extraction/examples/elm-extract/Fold.elm" Compute wrapped foldl_syn
          (Preambule "Fold")
@@ -116,5 +172,39 @@ Module ElmExamples.
          (Preambule "Increment")
          (main_and_test "Expect.equal (inc_counter O (Exist (S O))) (Exist (S O))").
 
+
+  MetaCoq Quote Recursively Definition last_syn := List.last.
+
+  Redirect "./extraction/examples/elm-extract/Last.elm" Compute wrapped last_syn
+          (Preambule "Last")
+          (main_and_test "Expect.equal (last (Cons 1 (Cons 10 Nil)) 0) 10").
+
+
+  Lemma O_gt_False : 0 > 0 -> False.
+  Proof. intros H;inversion H. Qed.
+
+  Program Definition safe_head {A} (non_empty_list : {l : list A | length l > 0}) : A :=
+    match non_empty_list as l' return l' = non_empty_list -> A  with
+    | [] => fun _ => False_rect _ _
+    | hd :: tl => fun _ => hd
+    end eq_refl.
+  Next Obligation.
+    intros. destruct non_empty_list as [l H1]. cbn in *;subst.
+    apply O_gt_False;auto.
+  Qed.
+
+  Program Definition head_of_repeat_2 {A} (a : A) := safe_head (repeat a 2).
+  Next Obligation.
+    intros. cbn. auto.
+  Qed.
+
+  MetaCoq Run (t <- tmQuoteRecTransp (@head_of_repeat_2) false ;;
+               tmDefinition "head_of_repeat_2_syn" t).
+
+  Redirect "./extraction/examples/elm-extract/SafeHead.elm"
+           Compute general_wrapped head_of_repeat_2_syn
+          (Preambule "SafeHead" ++ nl ++ elm_false_rec)
+          (main_and_test "Expect.equal (head_of_repeat_2 1) 1")
+          [<%% False_rect %%>] [(<%% False_rect %%>, "false_rec ()")].
 
 End ElmExamples.
